Redefined LLBC's semantics, and perform a reduction proof.

src/LLBC.v
@@ -5,17 +5,17 @@ Require Import List.
 Import ListNotations.
 Require Import PeanoNat.
 
-Variant LLBC_zero :=
+Inductive LLBC_val :=
 | LLBC_bot
 | LLBC_int (n : nat) (* TODO: use Aeneas integer types? *)
-| LLBC_loan (l : loan_id).
-
-Variant LLBC_unit :=
-| LLBC_borrow (l : loan_id).
-
-Variant LLBC_bin := .
-
-Notation LLBC_val := (value LLBC_zero LLBC_unit LLBC_bin).
+| LLBC_mut_loan (l : loan_id)
+| LLBC_mut_borrow (l : loan_id) (v : LLBC_val)
+(*
+| LLBC_shr_loan (l : loan_id) (v : LLBC_val)
+| LLBC_shr_borrow (l : loan_id)
+ *)
+(* | LLBC_pair (v0 : LLBC_val) (v1 : LLBC_val) *)
+.
 
 Variant LLBC_binder :=
 | Var (v : var)
@@ -23,146 +23,402 @@ Variant LLBC_binder :=
 | Anon.
 
 Program Global Instance EqDec_binder : EqDec LLBC_binder.
-Next Obligation. repeat decide equality. Qed.
+Next Obligation. repeat decide equality. Defined.
 
-Notation LLBC_state := (state LLBC_zero LLBC_unit LLBC_bin LLBC_binder).
+Variant LLBC_constructor :=
+| LLBC_botC
+| LLBC_intC (n : nat)
+| LLBC_mut_loanC (l : loan_id)
+| LLBC_mut_borrowC (l : loan_id)
+.
 
-Declare Scope llbc_scope.
-Delimit Scope llbc_scope with llbc.
+Definition LLBC_arity c := match c with
+| LLBC_botC => 0
+| LLBC_intC _ => 0
+| LLBC_mut_loanC _ => 0
+| LLBC_mut_borrowC _ => 1
+end.
 
-(* TODO: move these reserved notations in a separate files, maybe something like semantics-base. *)
-   
-Reserved Notation "'bot'" (at level 50).
+Definition LLBC_get_constructor v := match v with
+| LLBC_bot => LLBC_botC
+| LLBC_int n => LLBC_intC n
+| LLBC_mut_loan l => LLBC_mut_loanC l
+| LLBC_mut_borrow l _ => LLBC_mut_borrowC l
+end.
+
+Definition LLBC_subvalues v := match v with
+| LLBC_bot => []
+| LLBC_int _ => []
+| LLBC_mut_loan _ => []
+| LLBC_mut_borrow _ v => [v]
+end.
+
+Definition LLBC_fold c vs := match c, vs with
+| LLBC_intC n, [] => LLBC_int n
+| LLBC_mut_loanC l, [] => LLBC_mut_loan l
+| LLBC_mut_borrowC l, [v] => LLBC_mut_borrow l v
+| _, _ => LLBC_bot
+end.
+
+Program Instance ValueHLPL : Value LLBC_val := {
+  constructors := LLBC_constructor;
+  arity := LLBC_arity;
+  get_constructor := LLBC_get_constructor;
+  subvalues := LLBC_subvalues;
+  fold_value := LLBC_fold;
+  bot := LLBC_bot;
+}.
+Next Obligation. destruct v; reflexivity. Qed.
+Next Obligation.
+destruct v; destruct w; inversion eq_constructor; inversion eq_subvalues; reflexivity.
+Qed.
+
+Next Obligation.
+  destruct c; (rewrite length_zero_iff_nil in H; rewrite H) ||
+              destruct (length_1_is_singleton H) as [? ->];
+              reflexivity.
+Qed.
+Next Obligation.
+  destruct c; (rewrite length_zero_iff_nil in H; rewrite H) ||
+              destruct (length_1_is_singleton H) as [? ->];
+              reflexivity.
+Qed.
+
+Definition LLBC_state := state LLBC_binder LLBC_val.
+
+Declare Scope hlpl_plus_scope.
+Delimit Scope hlpl_plus_scope with hlpl_plus.
+
+(* TODO: move in lang.v *)
+Reserved Notation "'bot'" (at level 0).
 Reserved Notation "'loan^m' l" (at level 50).
-Reserved Notation "'borrow^m' l v" (at level 50).
-Reserved Notation "'loc' l v" (at level 50).
-Reserved Notation "'ptr' l" (at level 50).
+Reserved Notation "'borrow^m' ( l , v )" (at level 50, l at next level, v at next level).
 
-Notation "'bot'" := (@vZero LLBC_zero LLBC_unit LLBC_bin LLBC_bot): llbc_scope.
-Notation "'loan^m' l" := (@vZero LLBC_zero LLBC_unit LLBC_bin (LLBC_loan l))
-  : llbc_scope.
-Notation "'borrow^m' l v" := (@vUnit LLBC_zero LLBC_unit LLBC_bin (LLBC_borrow l) v)
-  : llbc_scope.
+Notation "'bot'" := LLBC_bot: hlpl_plus_scope.
+Notation "'loan^m' l" := (LLBC_mut_loan l) : hlpl_plus_scope.
+Notation "'borrow^m' ( l  , v )" := (LLBC_mut_borrow l v) : hlpl_plus_scope.
 
-(* Bind Scope llbc_scope with LLBC_val. *)
-Open Scope llbc_scope.
+(* Bind Scope hlpl_plus_scope with LLBC_val. *)
+Open Scope hlpl_plus_scope.
 
-Global Instance Inhabited_LLBC_val : Inhabited LLBC_val := { default := bot }.
+Inductive eval_proj (S : LLBC_state) perm : proj -> spath -> spath -> Prop :=
+(* Coresponds to R-Deref-MutBorrow and W-Deref-MutBorrow in the article. *)
+| Eval_Deref_MutBorrow q l v
+    (imm_or_mut : perm <> Mov)
+    (get_q : S.[q] = borrow^m(l, v)) :
+    eval_proj S perm Deref q (q +++ [0])
+.
 
-Inductive eval_path : LLBC_state -> path -> permission -> spath -> spath -> Prop :=
-| Eval_nil s perm pi : eval_path s [] perm pi pi
-| Eval_deref_borrow_mut s p q l v r
-    (extract_q : s{{q}} = vUnit (LLBC_borrow l) v)
-    (eval_q : eval_path s p Mut (q +++ [0]) r) :
-    eval_path s (Deref :: p) Mut q r.
+(* TODO: eval_path represents a computation, that evaluates and accumulate the result over [...] *)
+Inductive eval_path (S : LLBC_state) perm : path -> spath -> spath -> Prop :=
+(* Corresponds to R-Base and W-Base in the article. *)
+| Eval_nil pi : eval_path S perm [] pi pi
+| Eval_cons proj P p q r: eval_proj S perm proj p q -> eval_path S perm P q r ->
+    eval_path S perm (proj :: P) p r.
 
-Lemma eval_path_valid (s : LLBC_state) p perm q r (valid_q : valid_spath s q) (eval_q_r : eval_path s p perm q r) :
+Lemma eval_proj_valid S perm proj q r (H : eval_proj S perm proj q r) : valid_spath S r.
+Proof.
+  induction H.
+  - apply valid_spath_app. split.
+    + apply get_not_bot_valid_spath. rewrite get_q. discriminate.
+    + rewrite get_q. econstructor; reflexivity || constructor.
+Qed.
+
+Lemma eval_path_valid (s : LLBC_state) P perm q r
+  (valid_q : valid_spath s q) (eval_q_r : eval_path s perm P q r) :
   valid_spath s r.
 Proof.
   induction eval_q_r.
   - assumption.
-  - apply IHeval_q_r. rewrite valid_spath_app. split; try assumption. rewrite extract_q.
-    constructor. constructor.
+  - apply IHeval_q_r. eapply eval_proj_valid. eassumption.
 Qed.
 
-Definition eval_place (s : LLBC_state) (p : place) (perm : permission) (r : spath) :=
-  exists i, find_index s (Var (fst p)) = Some i /\ eval_path s (snd p) perm (i, []) r.
+Notation eval_place S perm p r :=
+  (exists i, find_binder S (Var (fst p)) = Some i /\ eval_path S perm (snd p) (i, []) r).
 
-Lemma eval_place_valid s p perm r (H : eval_place s p perm r) : valid_spath s r.
+Lemma eval_place_valid s p perm pi (H : eval_place s perm p pi) : valid_spath s pi.
 Proof.
   destruct H as (? & ? & ?). eapply eval_path_valid; try eassumption.
-  eapply find_index_valid_spath. eassumption.
+  eapply find_binder_valid. eassumption.
 Qed.
 
 (* Setting up the definitions for judgements like "loan \notin v" or
-   "l is free". *)
-Definition state_contains (f : LLBC_val -> bool) (s : LLBC_state) :=
-  exists v, valid_spath s v /\ is_true (f (s{{v}})).
+   "l is fresh". *)
+Definition state_contains (H : LLBC_val -> Prop) (S : LLBC_state) :=
+  exists p, valid_spath S p /\ H (S.[p]).
 
-Definition value_contains (f : LLBC_val -> bool) (s : LLBC_val) :=
-  exists v, valid_vpath s v /\ is_true (f (s{{v}})).
+Definition value_contains (H : LLBC_val -> Prop) (v : LLBC_val) :=
+  exists p, valid_vpath v p /\ H (v.[[p]]).
 
-Definition is_loan (v : LLBC_val) := match v with
-| vZero (LLBC_loan l) => true
-| _ => false
-end.
+Definition is_loan (v : LLBC_val) :=
+  exists l, v = loan^m(l).
 Definition contains_loan := value_contains is_loan.
 
-Definition is_loan_id (l : loan_id) (v : LLBC_val)  := match v with
-| vZero (LLBC_loan l') => l' =? l
-| vUnit (LLBC_borrow l') w => l' =? l
-| _ => false
-end.
-(* TODO: rename "is_fresh" *)
-Definition is_free l s := ~state_contains (is_loan_id l) s.
+Definition is_mut_borrow (v : LLBC_val) := exists l w, v = borrow^m(l, w).
 
-Definition is_borrow (v : LLBC_val) := match v with
-| vUnit (LLBC_borrow l) w => true
-| _ => false
-end.
+Definition contains_outer_loan v :=
+  exists l p, v.[[p]] = loan^m(l) /\ (forall q, vprefix q p -> ~is_mut_borrow (v.[[q]])).
 
-Definition not_in_borrow (s : LLBC_state) p :=
-  forall q, prefix q p /\ is_true (is_borrow (s{{q}})) -> q = p.
+Variant is_loan_id (l : loan_id) : LLBC_val -> Prop  :=
+| Is_loan_id_loan : is_loan_id l (loan^m(l))
+| Is_loan_id_borrow w : is_loan_id l (borrow^m(l, w))
+.
+
+Definition is_fresh l S := ~state_contains (is_loan_id l) S.
+
+Definition is_borrow (v : LLBC_val) := exists l w, v = borrow^m(l, w).
+
+Definition not_in_borrow (S : LLBC_state) p :=
+  forall q, prefix q p /\ is_borrow (S.[q]) -> q = p.
+
+Definition contains_bot (v : LLBC_val) :=
+  value_contains (fun w => w = bot) v.
 
 Inductive copy_val : LLBC_val -> LLBC_val -> Prop :=
-| Copy_val_int (n : nat) : copy_val (vZero (LLBC_int n)) (vZero (LLBC_int n)).
+| Copy_val_int (n : nat) : copy_val (LLBC_int n) (LLBC_int n)
+.
 
-Variant eval_op : LLBC_state -> operand -> LLBC_val -> LLBC_state -> Prop :=
-| Eval_IntConst s n : eval_op s (IntConst n) (vZero (LLBC_int n)) s
-(* TODO: place should be read in Imm mode. *)
-| Eval_copy s (p : place) q v : eval_place s p Mut q -> copy_val (s{{q}}) v ->
-    eval_op s (Copy p) v s
-(* TODO: s{{q}} cannot contain bot *)
-| Eval_move s (p : place) q : eval_place s p Mov q -> ~contains_loan (s{{q}}) ->
-    eval_op s (Move p) (s{{q}}) (s{{q <- bot}}).
+Variant eval_op (S : LLBC_state) : operand -> LLBC_val -> LLBC_state -> Prop :=
+| Eval_IntConst n : eval_op S (IntConst n) (LLBC_int n) S
+| Eval_copy (p : place) pi v : eval_place S Imm p pi -> copy_val (S.[pi]) v ->
+    eval_op S (Copy p) v S
+| Eval_move (p : place) pi : eval_place S Mov p pi -> ~contains_loan (S.[pi]) -> ~contains_bot (S.[pi]) ->
+  eval_op S (Move p) (S.[pi]) (S.[pi <- bot]).
 
-Variant eval_rvalue : LLBC_state -> rvalue -> LLBC_val -> LLBC_state -> Prop :=
-| Eval_just s op v s' : eval_op s op v s' -> eval_rvalue s (Just op) v s'
+Variant eval_rvalue (S : LLBC_state) : rvalue -> LLBC_val -> LLBC_state -> Prop :=
+| Eval_just op v S' : eval_op S op v S' -> eval_rvalue S (Just op) v S'
 (* For the moment, the only operation is the natural sum. *)
-| Eval_bin_op s s' s'' op_l op_r m n : eval_op s op_l (vZero (LLBC_int m)) s' ->
-   eval_op s' op_r (vZero (LLBC_int n)) s'' ->
-   eval_rvalue s (BinOp op_l op_r) (vZero (LLBC_int (m + n))) s''
-| Eval_borrow_m s p q l : eval_place s p Mut q -> ~contains_loan (s{{q}}) -> is_free l s ->
-    eval_rvalue s (&mut p) (vUnit (LLBC_borrow l) (s{{q}})) (s{{q <- vZero (LLBC_loan l)}}).
+| Eval_bin_op S' S'' op_l op_r m n : eval_op S op_l (LLBC_int m) S' ->
+   eval_op S' op_r (LLBC_int n) S'' ->
+   eval_rvalue S (BinOp op_l op_r) (LLBC_int (m + n)) S''
+| Eval_mut_borrow p pi l : eval_place S Mut p pi ->
+    ~contains_loan (S.[pi]) -> ~contains_bot (S.[pi]) -> is_fresh l S ->
+    eval_rvalue S (&mut p) (borrow^m(l, S.[pi])) (S.[pi <- loan^m(l)]).
 
 Inductive reorg : LLBC_state -> LLBC_state -> Prop :=
-| Reorg_refl s : reorg s s
-| Reorg_trans s0 s1 s2 : reorg s0 s1 -> reorg s1 s2 -> reorg s0 s2
-| Reorg_end_borrow_m s (p q : spath) l v : valid_spath s p -> valid_spath s q ->
-    s{{p}} = (vZero (LLBC_loan l)) -> s{{q}} = (vUnit (LLBC_borrow l) v) ->
-    ~contains_loan v -> not_in_borrow s q ->
-    reorg s (s{{p <- v}}{{q <- bot}}).
+| Reorg_none S : reorg S S
+| Reorg_seq S0 S1 S2 : reorg S0 S1 -> reorg S1 S2 -> reorg S0 S2
+| Reorg_end_borrow_m S (p q : spath) l v :
+    S.[p] = loan^m(l) -> S.[q] = borrow^m(l, v) ->
+    ~contains_loan v -> not_in_borrow S q ->
+    reorg S (S.[p <- v].[q <- bot]).
 
 (* When introducing non-terminating features (loops or recursivity), the signature of the relation
    is going to be:
    LLBC_state -> statement -> nat -> Option (statement_result * LLBC_state) -> Prop
 *)
 Inductive eval_stmt : LLBC_state -> statement -> statement_result -> LLBC_state -> Prop :=
-| Eval_nop s : eval_stmt s Nop rUnit s
+| Eval_nop S : eval_stmt S Nop rUnit S
 | Eval_seq_unit S0 S1 S2 stmt_l stmt_r r (eval_stmt_l : eval_stmt S0 stmt_l rUnit S1)
     (eval_stmt_r : eval_stmt S1 stmt_r r S2) : eval_stmt S0 (stmt_l ;; stmt_r) r S2
 | Eval_seq_panic S0 S1 stmt_l stmt_r (eval_stmt_l : eval_stmt S0 stmt_l rPanic S1) :
-    eval_stmt S0 (stmt_l ;; stmt_r) rPanic S1.
+    eval_stmt S0 (stmt_l ;; stmt_r) rPanic S1
+| Eval_assign S S' p rv v sp : eval_rvalue S rv v S' -> eval_place S' Mut p sp ->
+    ~contains_outer_loan (S'.[sp]) ->
+    eval_stmt S (ASSIGN p <- rv) rUnit ((Anon, S'.[sp]) :: S'.[sp <- v])
+| Eval_reorg S0 S1 S2 stmt r : reorg S0 S1 -> eval_stmt S1 stmt r S2 -> eval_stmt S0 stmt r S2.
 
-(* Can we actually relate the inductive properties to computable functions, in order to help
-   proving the evaluation of actual LLBC programs. *)
-Fixpoint eval_path_fun (s : LLBC_state) (p : path) perm (q : spath) : option spath :=
-match p with
-| [] => Some q
-| Deref :: p' => match s{{q}}, perm with
-  | vUnit (LLBC_borrow l) v, Mut => eval_path_fun s p' Mut (q +++ [0])
-  | _, _ => None
-  end
-| _ => None
-end.
+Require Import Bool.
+Local Open Scope option_monad_scope.
+(* Can we prove that the following proram terminates? *)
+(*
+fn main() {
+    let mut a = 1983;
+    let mut b = 1986;
+    let mut c = &mut a;
+    let d = &mut *c;
+    c = &mut b;
+    *d = 58;
+}
+ *)
+Definition a : var := 0.
+Definition b : var := 1.
+Definition c : var := 2.
+Definition d : var := 3.
+Definition main : statement :=
+  ASSIGN (a, []) <- Just (IntConst 1983) ;;
+  ASSIGN (b, []) <- Just (IntConst 1986) ;;
+  ASSIGN (c, []) <- &mut (a, []) ;;
+  ASSIGN (d, []) <- &mut (c, [Deref]) ;;
+  ASSIGN (c, []) <- &mut (b, []) ;;
+  ASSIGN (d, [Deref]) <- Just (IntConst 58) ;;
+  Nop
+.
+(* Important note: the line `c = &mut b` overwrites a loan, but as it is an outer loan, it doesn't
+ * cause any problem. This is a check that the overwriting of outer loans is supported. *)
+(* Also, the last `Nop` statement was added so that we could perform reorganization operations
+ * before the end, and but back the value 58 in the variable a. *)
 
-Lemma eval_path_fun_is_eval_path s p perm r : forall q,
-  eval_path_fun s p perm q = Some r -> eval_path s p perm q r.
+Notation init_state := [(Var a, bot); (Var b, bot); (Var c, bot); (Var d, bot)].
+
+Definition decide_contains_outer_loan v :=
+  match v with
+  | loan^m(l) => true
+  | _ => false
+  end.
+
+(* TODO: move in PathToSubtree.v *)
+Lemma valid_vpath_no_subvalues v p (valid_p : valid_vpath v p) (H : subvalues v = []) : p = [].
 Proof.
-  induction p as [ | proj]; intros q H.
-  - injection H. intros <-. constructor.
-  - destruct proj.
-    + simpl in H. destruct (extract_state Inhabited_LLBC_val s q) eqn:EQN; try easy. destruct l.
-      destruct perm; try easy. econstructor. exact EQN. auto.
-    + inversion H.
+  induction valid_p as [ | ? ? ? ? G].
+  - reflexivity.
+  - rewrite H, nth_error_nil in G. inversion G.
+Qed.
+
+(* For the moment, the type of values is so restricted that a value contains an outer loan if and
+ * only if it is a mutable loan. *)
+Lemma decide_contains_outer_loan_correct v :
+  contains_outer_loan v -> is_true (decide_contains_outer_loan v).
+Proof.
+  intros (l & p & H & G).
+  assert (valid_p : valid_vpath v p). { apply get_not_bot_valid_vpath. rewrite H. discriminate. }
+  destruct v.
+  - rewrite (valid_vpath_no_subvalues bot p) in H by auto. inversion H.
+  - erewrite (valid_vpath_no_subvalues _ p) in H by eauto. inversion H.
+  - auto.
+  - exfalso. apply (G []).
+    + exists p. reflexivity.
+    + repeat eexists.
+Qed.
+
+Definition decide_is_bot v := match v with bot => true | _ => false end.
+Definition decide_is_loan v := match v with loan^m(l) => true | _ => false end.
+Definition decide_is_loan_id l v :=
+  match v with
+  | borrow^m(l', _) | loan^m(l') => l =? l'
+  | _ => false
+  end.
+
+Fixpoint decide_value_contains (P : LLBC_val -> bool) v :=
+  P v || match v with borrow^m(l, w) => decide_value_contains P w | _ => false end.
+
+Lemma decide_value_contains_subval P v w i
+  (H : nth_error (subvalues v) i = Some w) (G : decide_value_contains P w = true) :
+  decide_value_contains P v = true.
+Proof.
+  apply nth_error_In in H.
+  destruct v; cbn in H; repeat destruct H as [<- | H] || destruct H.
+  cbn. rewrite G. apply orb_true_r.
+Qed.
+
+(* split in two lemmas. *)
+Lemma decide_value_contains_correct H P v (H_implies_P : forall v, H v -> P v = true) :
+  value_contains H v -> decide_value_contains P v = true.
+Proof.
+  intros (p & valid_p & H_v). induction valid_p as [ | ? ? ? ? G].
+  - apply H_implies_P in H_v. destruct v; cbn in *; rewrite H_v; reflexivity.
+  - apply (decide_value_contains_subval _ _ _ _ G). cbn in *. rewrite G in H_v. auto.
+Qed.
+
+Corollary decide_contains_bot v (H : contains_bot v) :
+  decide_value_contains decide_is_bot v = true.
+Proof. eapply decide_value_contains_correct; try exact H. intros ? ->. reflexivity. Qed.
+
+Corollary decide_contains_loan v (H : contains_loan v) :
+  decide_value_contains decide_is_loan v = true.
+Proof. eapply decide_value_contains_correct; try exact H. intros ? (? & ->). reflexivity. Qed.
+
+Definition decide_state_contains (P : LLBC_val -> bool) (S : LLBC_state) :=
+  existsb (fun bv => decide_value_contains P (snd bv)) S.
+
+Lemma decide_state_contains_correct H P S (H_implies_P : forall v, H v -> P v = true) :
+  state_contains H S -> decide_state_contains P S = true.
+Proof.
+  intros (p & (v & G & valid_p_v) & ?). apply existsb_exists.
+  unfold sget in *. destruct (nth_error S (fst p)) as [bv | ] eqn:EQN; inversion G.
+  exists bv. split.
+  - eapply nth_error_In. exact EQN.
+  - apply (decide_value_contains_correct _ _ _ H_implies_P). exists (snd p). subst. auto.
+Qed.
+
+Corollary decide_not_is_fresh S l (H : state_contains (is_loan_id l) S) :
+  decide_state_contains (decide_is_loan_id l) S = true.
+Proof.
+  eapply decide_state_contains_correct; try eassumption.
+  intros ? [ | ]; apply Nat.eqb_refl.
+Qed.
+
+(* TODO: move in PathToSubtree.v? *)
+Lemma prefix_nil p i : prefix p (i, []) -> p = (i, []).
+Proof.
+  destruct p as (j & q). intros (r & H). unfold app_spath_vpath in H. cbn in H.
+  apply pair_equal_spec in H. destruct H as (-> & H).
+  apply app_eq_nil in H. destruct H as (-> & _). reflexivity.
+Qed.
+  
+Lemma safe_main :
+  exists end_state, eval_stmt init_state main rUnit end_state /\
+    exists pi, eval_place end_state Imm ((a, []) : place) pi /\ end_state.[pi] = LLBC_int 58.
+Proof.
+  eexists. split. {
+    eapply Eval_seq_unit.
+    { apply Eval_assign.
+      - apply Eval_just, Eval_IntConst.
+      - eexists. split; reflexivity || econstructor.
+      - cbn. intro H. apply decide_contains_outer_loan_correct in H. inversion H.
+    }
+    cbn. eapply Eval_seq_unit.
+    { apply Eval_assign.
+      - apply Eval_just, Eval_IntConst.
+      - eexists. split; reflexivity || econstructor.
+      - cbn. intro H. apply decide_contains_outer_loan_correct in H. inversion H.
+    }
+    cbn. eapply Eval_seq_unit.
+    { apply Eval_assign.
+      - apply Eval_mut_borrow with (l := 0).
+        + eexists. split; reflexivity || econstructor.
+        + cbn. intro H. apply decide_contains_loan in H. discriminate H.
+        + cbn. intro H. apply decide_contains_bot in H. discriminate H.
+        + cbn. intro H. apply decide_not_is_fresh in H. discriminate H. 
+      - eexists. split; reflexivity || econstructor.
+      - cbn. intro H. apply decide_contains_outer_loan_correct in H. inversion H.
+    }
+    cbn. eapply Eval_seq_unit.
+    { apply Eval_assign.
+      - apply Eval_mut_borrow with (pi := (5, [0])) (l := 1).
+        + eexists. split; reflexivity || (repeat econstructor || discriminate). 
+        + cbn. intro H. apply decide_contains_loan in H. discriminate H.
+        + cbn. intro H. apply decide_contains_bot in H. discriminate H.
+        + cbn. intro H. apply decide_not_is_fresh in H. discriminate H.
+      - eexists. split; reflexivity || econstructor.
+      - cbn. intro H. apply decide_contains_outer_loan_correct in H. inversion H.
+    }
+    cbn. eapply Eval_seq_unit.
+    { apply Eval_assign.
+      - apply Eval_mut_borrow with (pi := (5, [])) (l := 2).
+        + eexists. split; reflexivity || (repeat econstructor || discriminate). 
+        + cbn. intro H. apply decide_contains_loan in H. discriminate H.
+        + cbn. intro H. apply decide_contains_bot in H. discriminate H.
+        + cbn. intro H. apply decide_not_is_fresh in H. discriminate H.
+      - eexists. split; reflexivity || econstructor.
+      - cbn. intro H. apply decide_contains_outer_loan_correct in H. inversion H.
+    }
+    cbn. eapply Eval_seq_unit.
+    { eapply Eval_assign.
+      - apply Eval_just, Eval_IntConst.
+      - eexists. split; reflexivity || (repeat econstructor || discriminate).
+      - cbn. intro H. apply decide_contains_outer_loan_correct in H. inversion H.
+    }
+    cbn. eapply Eval_reorg.
+    { eapply Reorg_seq.
+      - apply Reorg_end_borrow_m with (p := (1, [0])) (q := (9, [])) (l := 1).
+        + reflexivity.
+        + reflexivity.
+        + intros (p & valid_p & is_loan).
+          apply valid_vpath_no_subvalues in valid_p; try reflexivity. subst.
+          destruct is_loan as (? & H). inversion H.
+        + intros q (? & _). apply prefix_nil. assumption.
+      - cbn. apply Reorg_end_borrow_m with (l := 0) (p := (6, [])) (q := (1, [])).
+        + reflexivity.
+        + reflexivity.
+        + intros (p & valid_p & is_loan).
+          apply valid_vpath_no_subvalues in valid_p; try reflexivity. subst.
+          destruct is_loan as (? & H). inversion H.
+        + intros q (? & _). apply prefix_nil. assumption.
+    }
+    cbn. apply Eval_nop.
+  }
+  eexists. split.
+  - eexists. split; reflexivity || constructor.
+  - cbn. reflexivity.
 Qed.
